Translation.v
@@ -98,7 +98,13 @@ Definition or (s : term) (t : term) := not (and (not s) (not t)).
 Definition equals (s : term) (t : term) := not (or (less_than s t) (less_than t s)).
 
 (* NEEDS TO BE CAPTURE-AVOIDING *)
-Definition seq (s : term) (t : term) := app (lam (shift_up 0 t)) s.
+Definition seq (s : term) (t : term) := app (lam (Lambda.shift true 0 t)) s.
+
+Notation "x == y" := (equals x y) (at level 60).
+
+Notation "c1 ;; c2" :=
+  (seq c1 c2) (at level 80, right associativity).
+
 
 Definition y_combinator := 
   lam (app (lam (app (var 1) (app (var 0) (var 0)))) (lam (app (var 1) (app (var 0) (var 0)))) ).
@@ -110,12 +116,10 @@ Definition while_fics := app y_combinator while_fun.
 
 Definition while (s : term) (t : term) := app (app while_fics s) t.
 
-Notation "x == y" := (equals x y) (at level 60).
-
-Notation "c1 ;; c2" :=
-  (seq c1 c2) (at level 80, right associativity).
 Notation "'WHILE' b 'DO' c 'DONE'" :=
   (while b c) (at level 80, right associativity).
+
+
 
 Definition read_code (thread : bool) (base : nat) (buf_size : nat) := 
   LOOP thread base ::= ZERO ;;
@@ -313,128 +317,128 @@ Fact new_write_subst : forall x v e1 e2 e3 thread base buf_size,
   new_write thread base buf_size (subst x v e1) (subst x v e2) (subst x v e3) = subst x v (new_write thread base buf_size e1 e2 e3).
 Proof. intros. simpl. assert (forall x, (x + 1 = S x)). intros. omega. repeat (rewrite H). destruct thread. simpl. auto. auto. Qed.
 
-Fixpoint shift_up_n_c n c e  :=
+Fixpoint shift_n_c b n c e  :=
   match n with
     | 0 => e
-    | S n => shift_up_n_c n c (shift_up c e)
+    | S n => shift_n_c b n c (Lambda.shift b c e)
   end.
 
-Definition shift_up_n n e := shift_up_n_c n 0 e.
+Definition shift_n b n e := shift_n_c b n 0 e.
 
-Fact shift_up_n_c_array : forall n c k, shift_up_n_c n c (array k) = array k.
+Fact shift_n_c_array : forall n c k b, shift_n_c b n c (array k) = array k.
 Proof. intros. generalize dependent k. generalize dependent c. induction n ; intros.
   + simpl. auto.
   + simpl. rewrite IHn. auto. Qed.
 
-Fact shift_up_n_c_num : forall n c k, shift_up_n_c n c (num k) = num k.
+Fact shift_n_c_num : forall n c k b, shift_n_c b n c (num k) = num k.
 Proof. intros. generalize dependent k. generalize dependent c. induction n ; intros.
   + simpl. auto.
   + simpl. rewrite IHn. auto. Qed.
 
-Fact shift_up_n_c_tru : forall n c, shift_up_n_c n c tru = tru.
+Fact shift_n_c_tru : forall n c b, shift_n_c b n c tru = tru.
 Proof. intros. generalize dependent c. induction n ; intros.
   + simpl. auto.
   + simpl. rewrite IHn. auto. Qed.
 
-Fact shift_up_n_c_fls : forall n c, shift_up_n_c n c fls = fls.
+Fact shift_n_c_fls : forall n c b, shift_n_c b n c fls = fls.
 Proof. intros. generalize dependent c. induction n ; intros.
   + simpl. auto.
   + simpl. rewrite IHn. auto. Qed.
 
-Fact shift_up_n_c_yunit : forall n c, shift_up_n_c n c yunit = yunit.
+Fact shift_n_c_yunit : forall n c b, shift_n_c b n c yunit = yunit.
 Proof. intros. generalize dependent c. induction n ; intros.
   + simpl. auto.
   + simpl. rewrite IHn. auto. Qed.
 
-Fact shift_up_n_c_plus : forall n c e1 e2, shift_up_n_c n c (plus e1 e2) = plus (shift_up_n_c n c e1) (shift_up_n_c n c e2).
+Fact shift_n_c_plus : forall n c e1 e2 b, shift_n_c b n c (plus e1 e2) = plus (shift_n_c b n c e1) (shift_n_c b n c e2).
 Proof. intros. generalize dependent c. generalize dependent e1. generalize dependent e2. induction n ; intros.
   + simpl. auto.
   + simpl. rewrite IHn. auto. Qed.
 
-Fact shift_up_n_c_minus : forall n c e1 e2, shift_up_n_c n c (minus e1 e2) = minus (shift_up_n_c n c e1) (shift_up_n_c n c e2).
+Fact shift_n_c_minus : forall n c e1 e2 b, shift_n_c b n c (minus e1 e2) = minus (shift_n_c b n c e1) (shift_n_c b n c e2).
 Proof. intros. generalize dependent c. generalize dependent e1. generalize dependent e2. induction n ; intros.
   + simpl. auto.
   + simpl. rewrite IHn. auto. Qed.
 
-Fact shift_up_n_c_modulo : forall n c e1 e2, shift_up_n_c n c (modulo e1 e2) = modulo (shift_up_n_c n c e1) (shift_up_n_c n c e2).
+Fact shift_n_c_modulo : forall n c e1 e2 b, shift_n_c b n c (modulo e1 e2) = modulo (shift_n_c b n c e1) (shift_n_c b n c e2).
 Proof. intros. generalize dependent c. generalize dependent e1. generalize dependent e2. induction n ; intros.
   + simpl. auto.
   + simpl. rewrite IHn. auto. Qed.
 
-Fact shift_up_n_c_less_than : forall n c e1 e2, shift_up_n_c n c (less_than e1 e2) = less_than (shift_up_n_c n c e1) (shift_up_n_c n c e2).
+Fact shift_n_c_less_than : forall n c e1 e2 b, shift_n_c b n c (less_than e1 e2) = less_than (shift_n_c b n c e1) (shift_n_c b n c e2).
 Proof. intros. generalize dependent c. generalize dependent e1. generalize dependent e2. induction n ; intros.
   + simpl. auto.
   + simpl. rewrite IHn. auto. Qed.
 
-Fact shift_up_n_c_and : forall n c e1 e2, shift_up_n_c n c (and e1 e2) = and (shift_up_n_c n c e1) (shift_up_n_c n c e2).
+Fact shift_n_c_and : forall n c e1 e2 b, shift_n_c b n c (and e1 e2) = and (shift_n_c b n c e1) (shift_n_c b n c e2).
 Proof. intros. generalize dependent c. generalize dependent e1. generalize dependent e2. induction n ; intros.
   + simpl. auto.
   + simpl. rewrite IHn. auto. Qed.
 
-Fact shift_up_n_c_read : forall n c e1 e2, shift_up_n_c n c (read e1 e2) = read (shift_up_n_c n c e1) (shift_up_n_c n c e2).
+Fact shift_n_c_read : forall n c e1 e2 b, shift_n_c b n c (read e1 e2) = read (shift_n_c b n c e1) (shift_n_c b n c e2).
 Proof. intros. generalize dependent c. generalize dependent e1. generalize dependent e2. induction n ; intros.
   + simpl. auto.
   + simpl. rewrite IHn. auto. Qed.
 
-Fact shift_up_n_c_app : forall n c e1 e2, shift_up_n_c n c (app e1 e2) = app (shift_up_n_c n c e1) (shift_up_n_c n c e2).
+Fact shift_n_c_app : forall n c e1 e2 b, shift_n_c b n c (app e1 e2) = app (shift_n_c b n c e1) (shift_n_c b n c e2).
 Proof. intros. generalize dependent c. generalize dependent e1. generalize dependent e2. induction n ; intros.
   + simpl. auto.
   + simpl. rewrite IHn. auto. Qed.
 
-Fact shift_up_n_c_write : forall n c e1 e2 e3, shift_up_n_c n c (write e1 e2 e3) = write (shift_up_n_c n c e1) (shift_up_n_c n c e2) (shift_up_n_c n c e3).
+Fact shift_n_c_write : forall n c e1 e2 e3 b, shift_n_c b n c (write e1 e2 e3) = write (shift_n_c b n c e1) (shift_n_c b n c e2) (shift_n_c b n c e3).
 Proof. intros. generalize dependent c. generalize dependent e1. generalize dependent e2. generalize dependent e3. induction n ; intros.
   + simpl. auto.
   + simpl. rewrite IHn. auto. Qed.
 
-Fact shift_up_n_c_case : forall n c e1 e2 e3, shift_up_n_c n c (case e1 e2 e3) = case (shift_up_n_c n c e1) (shift_up_n_c n c e2) (shift_up_n_c n c e3).
+Fact shift_n_c_case : forall n c e1 e2 e3 b, shift_n_c b n c (case e1 e2 e3) = case (shift_n_c b n c e1) (shift_n_c b n c e2) (shift_n_c b n c e3).
 Proof. intros. generalize dependent c. generalize dependent e1. generalize dependent e2. generalize dependent e3. induction n ; intros.
   + simpl. auto.
   + simpl. rewrite IHn. auto. Qed.
 
-Fact shift_up_n_c_paire : forall n c e1 e2, shift_up_n_c n c (paire e1 e2) = paire (shift_up_n_c n c e1) (shift_up_n_c n c e2).
+Fact shift_n_c_paire : forall n c e1 e2 b, shift_n_c b n c (paire e1 e2) = paire (shift_n_c b n c e1) (shift_n_c b n c e2).
 Proof. intros. generalize dependent c. generalize dependent e1. generalize dependent e2. induction n ; intros.
   + simpl. auto.
   + simpl. rewrite IHn. auto. Qed.
 
-Fact shift_up_n_c_cast : forall n c e, shift_up_n_c n c (cast e) = cast (shift_up_n_c n c e).
+Fact shift_n_c_cast : forall n c e b, shift_n_c b n c (cast e) = cast (shift_n_c b n c e).
 Proof. intros. generalize dependent c. generalize dependent e. induction n ; intros.
   + simpl. auto.
   + simpl. rewrite IHn. auto. Qed.
 
-Fact shift_up_n_c_not : forall n c e, shift_up_n_c n c (not e) = not (shift_up_n_c n c e).
+Fact shift_n_c_not : forall n c e b, shift_n_c b n c (not e) = not (shift_n_c b n c e).
 Proof. intros. generalize dependent c. generalize dependent e. induction n ; intros.
   + simpl. auto.
   + simpl. rewrite IHn. auto. Qed.
 
-Fact shift_up_n_c_reference : forall n c e, shift_up_n_c n c (reference e) = reference (shift_up_n_c n c e).
+Fact shift_n_c_reference : forall n c e b, shift_n_c b n c (reference e) = reference (shift_n_c b n c e).
 Proof. intros. generalize dependent c. generalize dependent e. induction n ; intros.
   + simpl. auto.
   + simpl. rewrite IHn. auto. Qed.
 
-Fact shift_up_n_c_first : forall n c e, shift_up_n_c n c (first e) = first (shift_up_n_c n c e).
+Fact shift_n_c_first : forall n c e b, shift_n_c b n c (first e) = first (shift_n_c b n c e).
 Proof. intros. generalize dependent c. generalize dependent e. induction n ; intros.
   + simpl. auto.
   + simpl. rewrite IHn. auto. Qed.
 
-Fact shift_up_n_c_second : forall n c e, shift_up_n_c n c (second e) = second (shift_up_n_c n c e).
+Fact shift_n_c_second : forall n c e b, shift_n_c b n c (second e) = second (shift_n_c b n c e).
 Proof. intros. generalize dependent c. generalize dependent e. induction n ; intros.
   + simpl. auto.
   + simpl. rewrite IHn. auto. Qed.
 
 
-Fact shift_up_n_c_lam : forall n c e, shift_up_n_c n c (lam e) = lam (shift_up_n_c n (c+1) e).
+Fact shift_n_c_lam : forall n c e b, shift_n_c b n c (lam e) = lam (shift_n_c b n (c+1) e).
 Proof. intros. generalize dependent e. generalize dependent c. induction n ; intros.
   + simpl. auto.
   + simpl. rewrite IHn. auto. Qed.
 
-Fact shift_up_n_c_var1 : forall n c k, k < c -> shift_up_n_c n c (var k) = var k.
+Fact shift_n_c_var1 : forall n c k b, k < c -> shift_n_c b n c (var k) = var k.
 Proof. intros. generalize dependent k. generalize dependent c. induction n ; intros.
   + simpl. auto.
   + simpl. destruct (k <? c) eqn:ORIG.
     ++ apply Nat.ltb_lt in ORIG. apply IHn. auto.
     ++ apply Nat.ltb_lt in H. rewrite H in ORIG. inversion ORIG. Qed.
 
-Fact shift_up_n_c_var2 : forall n c k, k >= c -> shift_up_n_c n c (var k) = var (n+k).
+Fact shift_n_c_var2 : forall n c k , k >= c -> shift_n_c true n c (var k) = var (n+k).
 Proof. intros. generalize dependent k. generalize dependent c. induction n ; intros.
   + simpl. auto.
   + simpl. destruct (k <? c) eqn:ORIG.
@@ -442,100 +446,119 @@ Proof. intros. generalize dependent k. generalize dependent c. induction n ; int
     ++ rewrite IHn. assert (n+(k+1) = S(n+k)). omega. rewrite H0. auto. omega. Qed.
 
 
-Fact shift_up_n_eq : forall n c e, shift_up_n_c (n + 1) c e = shift_up (n+c) (shift_up_n_c n c e).
+Fact shift_n_c_var3 : forall n c k , k >= c -> shift_n_c false (S n) c (var k) = var (max (k-(S n)) (c-1)).
+Proof. intros. generalize dependent k. generalize dependent c. induction n ; intros.
+  + simpl. replace (max (k-1) (c-1)) with (k-1). destruct (k <? c) eqn:ORIG. apply Nat.ltb_lt in ORIG. omega. auto. symmetry. apply max_l. omega.
+  + replace (shift_n_c false (S (S n)) c (var k)) with (shift_n_c false (S n) c (Lambda.shift false c (var k))). simpl (Lambda.shift false c (var k)).
+destruct (k <? c) eqn:ORIG.
+    ++ apply Nat.ltb_lt in ORIG. omega.
+    ++ destruct (k =? c) eqn:ORIG2.
+       +++ apply beq_nat_true in ORIG2. subst. assert (forall n c, shift_n_c false n c (var (c-1)) = var (c-1)). intros. induction n0. simpl. auto. simpl. destruct (c0 - 1 <? c0) eqn:ORIG1. apply Nat.ltb_lt in ORIG1. auto. destruct c0. simpl in *. auto.
+assert (S c0 - 1 < S c0). omega. apply Nat.ltb_lt in H0. rewrite ORIG1 in H0.  inversion H0. rewrite H0. replace (max (c - S (S n)) (c-1)) with (c-1). auto. symmetry. apply max_r. omega.
+       +++ apply beq_nat_false in ORIG2. assert (k > c). omega. rewrite IHn. replace (k-1-S n) with (k-S(S n)). auto. omega. omega.
+    ++ simpl. auto. Qed.
+
+
+Fact shift_up_n_eq : forall n c e, shift_n_c true (n + 1) c e = Lambda.shift true (n+c) (shift_n_c true n c e).
 Proof. intros. generalize dependent c. generalize dependent n. induction e ; intros.
-  + rewrite shift_up_n_c_array. rewrite shift_up_n_c_array. simpl. auto.
-  + rewrite shift_up_n_c_num. rewrite shift_up_n_c_num. simpl. auto.
-  + rewrite shift_up_n_c_plus. rewrite shift_up_n_c_plus. rewrite IHe1. rewrite IHe2. simpl. auto.
-  + rewrite shift_up_n_c_minus. rewrite shift_up_n_c_minus. rewrite IHe1. rewrite IHe2. simpl. auto.
-  + rewrite shift_up_n_c_modulo. rewrite shift_up_n_c_modulo. rewrite IHe1. rewrite IHe2. simpl. auto.
-  + rewrite shift_up_n_c_tru. rewrite shift_up_n_c_tru. simpl. auto.
-  + rewrite shift_up_n_c_fls. rewrite shift_up_n_c_fls. simpl. auto.
-  + rewrite shift_up_n_c_less_than. rewrite shift_up_n_c_less_than. rewrite IHe1. rewrite IHe2. simpl. auto. 
-  + rewrite shift_up_n_c_not. rewrite shift_up_n_c_not. rewrite IHe. simpl. auto.
-  + rewrite shift_up_n_c_and. rewrite shift_up_n_c_and. rewrite IHe1. rewrite IHe2. simpl. auto.
-  + rewrite shift_up_n_c_yunit. rewrite shift_up_n_c_yunit. simpl. auto.
-  + rewrite shift_up_n_c_read. rewrite shift_up_n_c_read. rewrite IHe1. rewrite IHe2. simpl. auto.
-  + rewrite shift_up_n_c_write. rewrite shift_up_n_c_write. rewrite IHe1. rewrite IHe2. rewrite IHe3. simpl. auto.
-  + rewrite shift_up_n_c_reference. rewrite shift_up_n_c_reference. rewrite IHe. simpl. auto.
-  + rewrite shift_up_n_c_cast. rewrite shift_up_n_c_cast. rewrite IHe. simpl. auto.
-  + rewrite shift_up_n_c_case. rewrite shift_up_n_c_case. rewrite IHe1. rewrite IHe2. rewrite IHe3. simpl. auto.
-  + destruct (n <? c) eqn:ORIG. apply Nat.ltb_lt in ORIG. rewrite shift_up_n_c_var1. rewrite shift_up_n_c_var1. simpl. destruct (n <? n0 + c) eqn:ORIG1. apply Nat.ltb_lt in ORIG1. auto. assert (n < n0 + c -> False). intros. apply Nat.ltb_lt in H. rewrite H in ORIG1. inversion ORIG1. contradiction H. omega. auto. auto. assert (n <  c -> False). intros. apply Nat.ltb_lt in H. rewrite ORIG in H. inversion H. assert (n >= c). omega. rewrite shift_up_n_c_var2. rewrite shift_up_n_c_var2. simpl. destruct (n0 + n <? n0 + c) eqn:ORIG1. rewrite Nat.ltb_lt in ORIG1. omega. assert (n0+1+n=n0+n+1). omega. rewrite H1. auto. auto. auto.
-  + rewrite shift_up_n_c_app. rewrite shift_up_n_c_app. rewrite IHe1. rewrite IHe2. simpl. auto.
-  + rewrite shift_up_n_c_lam. rewrite shift_up_n_c_lam. assert (n+1=S n). omega. repeat (rewrite H in *). simpl. assert (shift_up_n_c (n + 1) (c+1) e =
-shift_up (n + (c + 1)) (shift_up_n_c n (c + 1) e)). apply IHe. assert (n+c+1=n+(c+1)). omega. rewrite H1 in *. rewrite <- H0. assert (n+1=S n). omega. rewrite H2 in *. simpl. auto.
-  + rewrite shift_up_n_c_paire. rewrite shift_up_n_c_paire. rewrite IHe1. rewrite IHe2. simpl. auto.
-  + rewrite shift_up_n_c_first. rewrite shift_up_n_c_first. rewrite IHe. simpl. auto.
-  + rewrite shift_up_n_c_second. rewrite shift_up_n_c_second. rewrite IHe. simpl. auto.
+  + rewrite shift_n_c_array. rewrite shift_n_c_array. simpl. auto.
+  + rewrite shift_n_c_num. rewrite shift_n_c_num. simpl. auto.
+  + rewrite shift_n_c_plus. rewrite shift_n_c_plus. rewrite IHe1. rewrite IHe2. simpl. auto.
+  + rewrite shift_n_c_minus. rewrite shift_n_c_minus. rewrite IHe1. rewrite IHe2. simpl. auto.
+  + rewrite shift_n_c_modulo. rewrite shift_n_c_modulo. rewrite IHe1. rewrite IHe2. simpl. auto.
+  + rewrite shift_n_c_tru. rewrite shift_n_c_tru. simpl. auto.
+  + rewrite shift_n_c_fls. rewrite shift_n_c_fls. simpl. auto.
+  + rewrite shift_n_c_less_than. rewrite shift_n_c_less_than. rewrite IHe1. rewrite IHe2. simpl. auto. 
+  + rewrite shift_n_c_not. rewrite shift_n_c_not. rewrite IHe. simpl. auto.
+  + rewrite shift_n_c_and. rewrite shift_n_c_and. rewrite IHe1. rewrite IHe2. simpl. auto.
+  + rewrite shift_n_c_yunit. rewrite shift_n_c_yunit. simpl. auto.
+  + rewrite shift_n_c_read. rewrite shift_n_c_read. rewrite IHe1. rewrite IHe2. simpl. auto.
+  + rewrite shift_n_c_write. rewrite shift_n_c_write. rewrite IHe1. rewrite IHe2. rewrite IHe3. simpl. auto.
+  + rewrite shift_n_c_reference. rewrite shift_n_c_reference. rewrite IHe. simpl. auto.
+  + rewrite shift_n_c_cast. rewrite shift_n_c_cast. rewrite IHe. simpl. auto.
+  + rewrite shift_n_c_case. rewrite shift_n_c_case. rewrite IHe1. rewrite IHe2. rewrite IHe3. simpl. auto.
+  + destruct (n <? c) eqn:ORIG. apply Nat.ltb_lt in ORIG. rewrite shift_n_c_var1. rewrite shift_n_c_var1. simpl. destruct (n <? n0 + c) eqn:ORIG1. apply Nat.ltb_lt in ORIG1. auto. assert (n < n0 + c -> False). intros. apply Nat.ltb_lt in H. rewrite H in ORIG1. inversion ORIG1. contradiction H. omega. auto. auto. assert (n <  c -> False). intros. apply Nat.ltb_lt in H. rewrite ORIG in H. inversion H. assert (n >= c). omega. rewrite shift_n_c_var2. rewrite shift_n_c_var2. simpl. destruct (n0 + n <? n0 + c) eqn:ORIG1. rewrite Nat.ltb_lt in ORIG1. omega. assert (n0+1+n=n0+n+1). omega. rewrite H1. auto. auto. auto.
+  + rewrite shift_n_c_app. rewrite shift_n_c_app. rewrite IHe1. rewrite IHe2. simpl. auto.
+  + rewrite shift_n_c_lam. rewrite shift_n_c_lam. assert (n+1=S n). omega. repeat (rewrite H in *). simpl. assert (shift_n_c true (n + 1) (c+1) e =
+Lambda.shift true (n + (c + 1)) (shift_n_c true n (c + 1) e)). apply IHe. assert (n+c+1=n+(c+1)). omega. rewrite H1 in *. rewrite <- H0. assert (n+1=S n). omega. rewrite H2 in *. simpl. auto.
+  + rewrite shift_n_c_paire. rewrite shift_n_c_paire. rewrite IHe1. rewrite IHe2. simpl. auto.
+  + rewrite shift_n_c_first. rewrite shift_n_c_first. rewrite IHe. simpl. auto.
+  + rewrite shift_n_c_second. rewrite shift_n_c_second. rewrite IHe. simpl. auto.
 Qed.
 
-Fact foo : forall n e, shift_up_n_c (S n) 0 e = shift_up 0 (shift_up_n_c n 0 e).
+Fact foo : forall n e b, shift_n_c b (S n) 0 e = Lambda.shift b 0 (shift_n_c b n 0 e).
 Proof. intros. generalize dependent e. induction n ; intros ; simpl.
   + auto.
   + rewrite <- IHn. simpl. auto. Qed.
 
-Fact blah : forall x v e c, subst (x + (c+1)) (shift_up_n (c+1) v) (shift_up c e) =
-shift_up c (subst (x + c) (shift_up_n c v) e).
-Proof. intros. generalize dependent x. generalize dependent v. generalize dependent c. induction e ; intros ; simpl ; try auto ; try (rewrite IHe1 ; rewrite IHe2 ; auto); try (rewrite IHe3 ; auto) ; try (rewrite IHe ; auto). destruct (n =? x + c) eqn:ORIG. apply beq_nat_true in ORIG. subst. destruct (x + c <? c) eqn:ORIG. rewrite Nat.ltb_lt in ORIG. omega. simpl. destruct (x + c + 1 =? x + (c + 1)) eqn:ORIG1. apply beq_nat_true in ORIG1. unfold shift_up_n. rewrite shift_up_n_eq. assert (c+0=c). omega. rewrite H. auto. apply beq_nat_false in ORIG1. contradiction ORIG1. omega. destruct (n <? c) eqn:ORIG1. apply Nat.ltb_lt in ORIG1. simpl. destruct ( n =? x + (c + 1)) eqn:ORIG2. apply beq_nat_true in ORIG2. subst. omega. destruct (n <? c) eqn:ORIG3. auto. assert ((n <? c) = true -> False). intros. rewrite ORIG3 in H. inversion H. assert ((n <? c) = true). apply Nat.ltb_lt. auto. apply H in H0. contradiction. simpl. destruct (n + 1 =? x + (c + 1)) eqn:ORIG2. apply beq_nat_true in ORIG2. assert (n=x+c). omega. subst. apply beq_nat_false in ORIG. contradiction ORIG. auto. destruct (n <? c) eqn:ORIG3. inversion ORIG1. auto. unfold shift_up_n in *. rewrite <- foo. rewrite <- foo. assert (x+(c+1)+1=x+((c+1)+1)). omega. rewrite H. clear H. assert (S (c+1) = (c+1)+1). omega. rewrite H. clear H. rewrite IHe. assert (x+(c+1)=x+c+1). omega. rewrite H. auto. clear H. assert (c+1=S c). omega. rewrite H. auto. Qed.
+Fact blah : forall x v e c, subst (x + (c+1)) (shift_n true (c+1) v) (Lambda.shift true c e) =
+Lambda.shift true c (subst (x + c) (shift_n true c v) e).
+Proof. intros. generalize dependent x. generalize dependent v. generalize dependent c. induction e ; intros ; simpl ; try auto ; try (rewrite IHe1 ; rewrite IHe2 ; auto); try (rewrite IHe3 ; auto) ; try (rewrite IHe ; auto). destruct (n =? x + c) eqn:ORIG. apply beq_nat_true in ORIG. subst. destruct (x + c <? c) eqn:ORIG. rewrite Nat.ltb_lt in ORIG. omega. simpl. destruct (x + c + 1 =? x + (c + 1)) eqn:ORIG1. apply beq_nat_true in ORIG1. unfold shift_n. rewrite shift_up_n_eq. assert (c+0=c). omega. rewrite H. auto. apply beq_nat_false in ORIG1. contradiction ORIG1. omega. destruct (n <? c) eqn:ORIG1. apply Nat.ltb_lt in ORIG1. simpl. destruct ( n =? x + (c + 1)) eqn:ORIG2. apply beq_nat_true in ORIG2. subst. omega. destruct (n <? c) eqn:ORIG3. auto. assert ((n <? c) = true -> False). intros. rewrite ORIG3 in H. inversion H. assert ((n <? c) = true). apply Nat.ltb_lt. auto. apply H in H0. contradiction. simpl. destruct (n + 1 =? x + (c + 1)) eqn:ORIG2. apply beq_nat_true in ORIG2. assert (n=x+c). omega. subst. apply beq_nat_false in ORIG. contradiction ORIG. auto. destruct (n <? c) eqn:ORIG3. inversion ORIG1. auto. unfold shift_n in *. rewrite <- foo. rewrite <- foo. assert (x+(c+1)+1=x+((c+1)+1)). omega. rewrite H. clear H. assert (S (c+1) = (c+1)+1). omega. rewrite H. clear H. rewrite IHe. assert (x+(c+1)=x+c+1). omega. rewrite H. auto. clear H. assert (c+1=S c). omega. rewrite H. auto. Qed.
 
 
-Fact helper : forall x v e, subst (x + 1) (shift_up 0 v) (shift_up 0 e) = shift_up 0 (subst x v e).
+Fact helper : forall x v e, subst (x + 1) (Lambda.shift true 0 v) (Lambda.shift true 0 e) = Lambda.shift true 0 (subst x v e).
 Proof. intros. intros. generalize dependent x. generalize dependent v. induction e ; intros ; simpl ; auto ; try (rewrite IHe1 ; rewrite IHe2 ; auto) ; try (rewrite IHe3 ; auto) ; try (rewrite IHe ; auto).
   + destruct (n + 1 =? x + 1) eqn:ORIG.
     ++ apply beq_nat_true in ORIG. assert (n=x). omega. subst. destruct (x =? x) eqn:ORIG1. auto. apply beq_nat_false in ORIG1. contradiction ORIG1. auto.
     ++ apply beq_nat_false in ORIG. assert (n <> x). omega. destruct (n =? x) eqn:ORIG1. apply beq_nat_true in ORIG1. subst. contradiction H. auto. simpl. auto.
-  + assert (shift_up 0 (shift_up 0 v) = shift_up_n_c (1+1) 0 v). rewrite foo. rewrite foo. simpl. auto. rewrite H. clear H. assert (shift_up_n_c (1 + 1) 0 v = shift_up_n (1+1) v). unfold shift_up_n. auto. rewrite H. clear H. assert (x+1+1=x+(1+1)). omega. rewrite H. rewrite blah.
-simpl. unfold shift_up_n. simpl. auto. Qed.
+  + assert (Lambda.shift true 0 (Lambda.shift true 0 v) = shift_n_c true (1+1) 0 v). rewrite foo. rewrite foo. simpl. auto. rewrite H. clear H. assert (shift_n_c true (1 + 1) 0 v = shift_n true (1+1) v). unfold shift_n. auto. rewrite H. clear H. assert (x+1+1=x+(1+1)). omega. rewrite H. rewrite blah.
+simpl. unfold shift_n. simpl. auto. Qed.
 
 Fact seq_subst : forall x v e e', subst x v (e;;e') = ((subst x v e) ;; (subst x v e')).
 Proof. intros. unfold seq. rewrite subst_app. rewrite subst_lam. rewrite helper. auto. Qed.
 
-Fact shift_up_flush_star1 : forall c thread base buf_size,
-  shift_up c(flush_star thread base buf_size) = flush_star thread base buf_size.
-Proof. intros. simpl. assert (forall x, (x + 1 = S x)). intros. omega. repeat (rewrite H). destruct thread. simpl. auto. auto. Qed.
+Fact shift_flush_star1 : forall c b thread base buf_size,
+  Lambda.shift b c (flush_star thread base buf_size) = flush_star thread base buf_size.
+Proof. intros. destruct b.
+  + simpl. assert (forall x, (x + 1 = S x)). intros. omega. repeat (rewrite H). destruct thread. simpl. auto. auto.
+  + simpl. assert (forall x, (x + 1 = S x)). intros. omega. repeat (rewrite H). destruct thread. simpl. auto. auto. Qed.
 
-Fact shift_up_new_read_star1 : forall c thread base buf_size e1 e2,
-  shift_up c (new_read thread base buf_size e1 e2) = new_read thread base buf_size  (shift_up c e1) (shift_up c e2).
-Proof. intros. unfold new_read. unfold read_code. simpl. assert (forall x, (x + 1 = S x)). intros. omega. repeat (rewrite H). destruct thread. simpl. auto. auto. Qed.
+Fact shift_new_read_star1 : forall c b thread base buf_size e1 e2,
+  Lambda.shift b c (new_read thread base buf_size e1 e2) = new_read thread base buf_size  (Lambda.shift b c e1) (Lambda.shift b c e2).
+Proof. intros. destruct b.
+  + unfold new_read. unfold read_code. simpl. assert (forall x, (x + 1 = S x)). intros. omega. repeat (rewrite H). destruct thread. simpl. auto. auto.
+  + unfold new_read. unfold read_code. simpl. assert (forall x, (x + 1 = S x)). intros. omega. repeat (rewrite H). destruct thread. simpl. auto. auto. Qed.
 
-Fact shift_up_new_write_star1 : forall c thread base buf_size e1 e2 e3,
-  shift_up c (new_write thread base buf_size e1 e2 e3) = new_write thread base buf_size  (shift_up c e1) (shift_up c e2) (shift_up c e3).
-Proof. intros. unfold new_write. unfold write_code. simpl. assert (forall x, (x + 1 = S x)). intros. omega. repeat (rewrite H). destruct thread. simpl. auto. auto. Qed.
+Fact shift_new_write_star1 : forall c b thread base buf_size e1 e2 e3,
+  Lambda.shift b c (new_write thread base buf_size e1 e2 e3) = new_write thread base buf_size  (Lambda.shift b c e1) (Lambda.shift b c e2) (Lambda.shift b c e3).
+Proof. intros. destruct b.
+  + unfold new_write. unfold write_code. simpl. assert (forall x, (x + 1 = S x)). intros. omega. repeat (rewrite H). destruct thread. simpl. auto. auto.
+  + unfold new_write. unfold write_code. simpl. assert (forall x, (x + 1 = S x)). intros. omega. repeat (rewrite H). destruct thread. simpl. auto. auto. Qed.
 
-Fact foo1 : forall c k e, shift_up (c + k + 1) (shift_up k e) = shift_up k (shift_up (c + k) e).
+Fact foo1 : forall c k e, Lambda.shift true (c + k + 1) (Lambda.shift true k e) = Lambda.shift true k (Lambda.shift true (c + k) e).
 Proof. intros. generalize dependent c. generalize dependent k. induction e ; intros ; simpl ; auto ; try (rewrite IHe1 ; rewrite IHe2 ; auto) ; try (rewrite IHe3 ; auto) ; try (rewrite IHe ; auto). 
   + destruct (n <? k) eqn:ORIG.
     ++ assert (COPY:=ORIG). apply Nat.ltb_lt in ORIG. assert (n  <? c + k = true). apply Nat.ltb_lt. omega. rewrite H. apply Nat.ltb_lt in H. simpl. rewrite COPY. assert (n <? c+k+1 = true). apply Nat.ltb_lt. omega. rewrite H0. auto.
     ++ simpl. destruct (n + 1 <? c + k + 1) eqn:ORIG1. apply Nat.ltb_lt in ORIG1. assert (n <? c+k = true). apply Nat.ltb_lt. omega. rewrite H. simpl. destruct (n <? k) eqn:ORIG2. inversion ORIG. auto. assert (n + 1 <? c + k + 1 = true -> False). intros. rewrite ORIG1 in H. inversion H. destruct (n <? c + k) eqn:ORIG2. contradiction H. apply Nat.ltb_lt. apply Nat.ltb_lt in ORIG2. omega. simpl. destruct (n + 1 <? k) eqn:ORIG3. apply Nat.ltb_lt in ORIG3. assert (n<k -> False). intros. apply Nat.ltb_lt in H0. rewrite ORIG in H0. inversion H0. clear ORIG1. contradiction H0. omega. auto.
   + assert (c+k+1+1=c+(k+1)+1). omega. rewrite H. rewrite IHe. assert (c+(k+1)=c+k+1). omega. rewrite H0. auto. Qed.
 
-Fact shift_up_seq : forall c e1 e2 , shift_up c (e1;;e2) = ((shift_up c e1);;(shift_up c e2)).
-Proof. intros. unfold seq. rewrite shift_up_app. rewrite shift_up_lam. assert (shift_up (c + 1) (shift_up 0 e2) = shift_up 0 (shift_up c e2)). assert (c+0+1=c+1). omega. rewrite <- H. rewrite foo1. assert (c+0=c). omega. rewrite H0. auto. rewrite H. auto. Qed.
+Fact shift_up_seq : forall c e1 e2 , Lambda.shift true c (e1;;e2) = ((Lambda.shift true c e1);;(Lambda.shift true c e2)).
+Proof. intros. unfold seq. rewrite shift_app. rewrite shift_lam. assert (Lambda.shift true (c + 1) (Lambda.shift true 0 e2) = Lambda.shift true 0 (Lambda.shift true c e2)). assert (c+0+1=c+1). omega. rewrite <- H. rewrite foo1. assert (c+0=c). omega. rewrite H0. auto. rewrite H. auto. Qed.
 
-Fact shift_commutes_with_translate : forall c e thread base buf_size, translate (shift_up c e) thread base buf_size = shift_up c (translate e thread base buf_size).
+Fact shift_up_commutes_with_translate : forall c e thread base buf_size, translate (Lambda.shift true c e) thread base buf_size = Lambda.shift true c (translate e thread base buf_size).
 Proof. intros. generalize dependent c; induction e ; intros.
   + simpl. auto.
   + simpl. auto.
-  + rewrite shift_up_plus. rewrite translate_plus. rewrite translate_plus. rewrite shift_up_app. rewrite shift_up_plus. rewrite shift_up_lam. rewrite shift_up_seq. rewrite shift_up_flush_star1. rewrite IHe1. rewrite IHe2. destruct c; simpl ; auto.
-  + rewrite shift_up_minus. rewrite translate_minus. rewrite translate_minus. rewrite shift_up_app. rewrite shift_up_minus. rewrite shift_up_lam. rewrite shift_up_seq. rewrite shift_up_flush_star1. rewrite IHe1. rewrite IHe2. simpl. destruct c; simpl ; auto.
-  + rewrite shift_up_modulo. rewrite translate_modulo. rewrite translate_modulo. rewrite shift_up_app. rewrite shift_up_modulo. rewrite shift_up_lam. rewrite shift_up_seq. rewrite shift_up_flush_star1. rewrite IHe1. rewrite IHe2. destruct c; simpl ; auto.
+  + rewrite shift_plus. rewrite translate_plus. rewrite translate_plus. rewrite shift_app. rewrite shift_plus. rewrite shift_lam. rewrite shift_up_seq. rewrite shift_flush_star1. rewrite IHe1. rewrite IHe2. destruct c; simpl ; auto.
+  + rewrite shift_minus. rewrite translate_minus. rewrite translate_minus. rewrite shift_app. rewrite shift_minus. rewrite shift_lam. rewrite shift_up_seq. rewrite shift_flush_star1. rewrite IHe1. rewrite IHe2. simpl. destruct c; simpl ; auto.
+  + rewrite shift_modulo. rewrite translate_modulo. rewrite translate_modulo. rewrite shift_app. rewrite shift_modulo. rewrite shift_lam. rewrite shift_up_seq. rewrite shift_flush_star1. rewrite IHe1. rewrite IHe2. destruct c; simpl ; auto.
   + simpl. auto.
   + simpl. auto.
-  + rewrite shift_up_less_than. rewrite translate_less_than. rewrite translate_less_than. rewrite shift_up_app. rewrite shift_up_less_than. rewrite shift_up_lam. rewrite shift_up_seq. rewrite shift_up_flush_star1. rewrite IHe1. rewrite IHe2. destruct c; simpl ; auto.
-  + rewrite shift_up_not. rewrite translate_not. rewrite translate_not. rewrite shift_up_app. rewrite shift_up_not. rewrite shift_up_lam. rewrite shift_up_seq. rewrite shift_up_flush_star1. rewrite IHe. destruct c; simpl ; auto.
-  + rewrite shift_up_and. rewrite translate_and. rewrite translate_and. rewrite shift_up_app. rewrite shift_up_and. rewrite shift_up_lam. rewrite shift_up_seq. rewrite shift_up_flush_star1. rewrite IHe1. rewrite IHe2. simpl. destruct c; simpl ; auto.
+  + rewrite shift_less_than. rewrite translate_less_than. rewrite translate_less_than. rewrite shift_app. rewrite shift_less_than. rewrite shift_lam. rewrite shift_up_seq. rewrite shift_flush_star1. rewrite IHe1. rewrite IHe2. destruct c; simpl ; auto.
+  + rewrite shift_not. rewrite translate_not. rewrite translate_not. rewrite shift_app. rewrite shift_not. rewrite shift_lam. rewrite shift_up_seq. rewrite shift_flush_star1. rewrite IHe. destruct c; simpl ; auto.
+  + rewrite shift_and. rewrite translate_and. rewrite translate_and. rewrite shift_app. rewrite shift_and. rewrite shift_lam. rewrite shift_up_seq. rewrite shift_flush_star1. rewrite IHe1. rewrite IHe2. simpl. destruct c; simpl ; auto.
   + simpl. auto.
-  + rewrite shift_up_read. rewrite translate_read. rewrite translate_read. rewrite shift_up_app. rewrite IHe1. rewrite IHe2. rewrite shift_up_new_read_star1. rewrite shift_up_lam. rewrite shift_up_seq. rewrite shift_up_flush_star1. destruct c; simpl ; auto.
-  + rewrite shift_up_write. rewrite translate_write. rewrite translate_write. rewrite shift_up_app. rewrite IHe1. rewrite IHe2. rewrite IHe3. rewrite shift_up_new_write_star1. rewrite shift_up_lam. rewrite shift_up_seq. rewrite shift_up_flush_star1. simpl (shift_up (0 + 1) (var 0)). destruct c; simpl ; auto.
-  + rewrite shift_up_reference. rewrite translate_reference. rewrite translate_reference. rewrite shift_up_app. rewrite shift_up_reference. rewrite shift_up_lam. rewrite shift_up_seq. rewrite shift_up_flush_star1. rewrite IHe. destruct c; simpl ; auto.
-  + rewrite shift_up_cast. rewrite translate_cast. rewrite translate_cast. rewrite shift_up_app. rewrite shift_up_cast. rewrite shift_up_lam. rewrite shift_up_seq. rewrite shift_up_flush_star1. rewrite IHe. destruct c; simpl ; auto.
-  + rewrite shift_up_case. rewrite translate_case. rewrite translate_case. rewrite shift_up_case. rewrite shift_up_seq. rewrite shift_up_flush_star1. rewrite shift_up_seq. rewrite shift_up_flush_star1. rewrite IHe1. rewrite IHe2. rewrite IHe3. destruct c; simpl ; auto.
+  + rewrite shift_read. rewrite translate_read. rewrite translate_read. rewrite shift_app. rewrite IHe1. rewrite IHe2. rewrite shift_new_read_star1. rewrite shift_lam. rewrite shift_up_seq. rewrite shift_flush_star1. destruct c; simpl ; auto.
+  + rewrite shift_write. rewrite translate_write. rewrite translate_write. rewrite shift_app. rewrite IHe1. rewrite IHe2. rewrite IHe3. rewrite shift_new_write_star1. rewrite shift_lam. rewrite shift_up_seq. rewrite shift_flush_star1. simpl (Lambda.shift true (0 + 1) (var 0)). destruct c; simpl ; auto.
+  + rewrite shift_reference. rewrite translate_reference. rewrite translate_reference. rewrite shift_app. rewrite shift_reference. rewrite shift_lam. rewrite shift_up_seq. rewrite shift_flush_star1. rewrite IHe. destruct c; simpl ; auto.
+  + rewrite shift_cast. rewrite translate_cast. rewrite translate_cast. rewrite shift_app. rewrite shift_cast. rewrite shift_lam. rewrite shift_up_seq. rewrite shift_flush_star1. rewrite IHe. destruct c; simpl ; auto.
+  + rewrite shift_case. rewrite translate_case. rewrite translate_case. rewrite shift_case. rewrite shift_up_seq. rewrite shift_flush_star1. rewrite shift_up_seq. rewrite shift_flush_star1. rewrite IHe1. rewrite IHe2. rewrite IHe3. destruct c; simpl ; auto.
   + simpl. destruct (n <? c); simpl ; auto.
-  + rewrite shift_up_app. rewrite translate_app. rewrite translate_app. rewrite shift_up_app. rewrite IHe1. rewrite IHe2. destruct c; simpl ; auto.
-  + rewrite shift_up_lam. rewrite translate_lam. rewrite translate_lam. rewrite shift_up_lam. rewrite shift_up_seq. rewrite shift_up_flush_star1. rewrite IHe. auto.
-  + rewrite shift_up_paire. rewrite translate_paire. rewrite translate_paire. rewrite shift_up_paire. rewrite IHe1. rewrite IHe2. destruct c; simpl ; auto.
-  + rewrite shift_up_first. rewrite translate_first. rewrite translate_first. rewrite shift_up_app. rewrite shift_up_first. rewrite shift_up_lam. rewrite shift_up_seq. rewrite shift_up_flush_star1. rewrite IHe. destruct c; simpl ; auto.
-  + rewrite shift_up_second. rewrite translate_second. rewrite translate_second. rewrite shift_up_app. rewrite shift_up_second. rewrite shift_up_lam. rewrite shift_up_seq. rewrite shift_up_flush_star1. rewrite IHe. destruct c; simpl ; auto. Qed.
+  + rewrite shift_app. rewrite translate_app. rewrite translate_app. rewrite shift_app. rewrite IHe1. rewrite IHe2. destruct c; simpl ; auto.
+  + rewrite shift_lam. rewrite translate_lam. rewrite translate_lam. rewrite shift_lam. rewrite shift_up_seq. rewrite shift_flush_star1. rewrite IHe. auto.
+  + rewrite shift_paire. rewrite translate_paire. rewrite translate_paire. rewrite shift_paire. rewrite IHe1. rewrite IHe2. destruct c; simpl ; auto.
+  + rewrite shift_first. rewrite translate_first. rewrite translate_first. rewrite shift_app. rewrite shift_first. rewrite shift_lam. rewrite shift_up_seq. rewrite shift_flush_star1. rewrite IHe. destruct c; simpl ; auto.
+  + rewrite shift_second. rewrite translate_second. rewrite translate_second. rewrite shift_app. rewrite shift_second. rewrite shift_lam. rewrite shift_up_seq. rewrite shift_flush_star1. rewrite IHe. destruct c; simpl ; auto. Qed.
 
 Fact seq_flush_subst : forall x v thread base buf_size e, subst x v (flush_star thread base buf_size;; e) =  (flush_star thread base buf_size;; (subst x v e)).
 Proof. intros. rewrite seq_subst. rewrite subst_flush_star1. auto. Qed.
@@ -561,7 +584,7 @@ Proof. intros. generalize dependent v. generalize dependent x. induction e ; int
   + rewrite subst_case. rewrite translate_case. rewrite translate_case. rewrite subst_case. rewrite IHe1. rewrite IHe2. rewrite IHe3. rewrite seq_flush_subst. rewrite seq_flush_subst. auto.
   + rewrite subst_var. simpl. destruct (n =? x). auto. simpl. auto.
   + rewrite subst_app. rewrite translate_app. rewrite IHe1. rewrite IHe2. reflexivity.
-  + rewrite subst_lam. rewrite translate_lam. rewrite translate_lam. rewrite subst_lam. rewrite seq_subst. rewrite subst_flush_star1. rewrite IHe. rewrite shift_commutes_with_translate. auto.
+  + rewrite subst_lam. rewrite translate_lam. rewrite translate_lam. rewrite subst_lam. rewrite seq_subst. rewrite subst_flush_star1. rewrite IHe. rewrite shift_up_commutes_with_translate. auto.
   + rewrite subst_paire. rewrite translate_paire. rewrite translate_paire. rewrite subst_paire. rewrite IHe1. rewrite IHe2. reflexivity.
   + rewrite subst_first. rewrite translate_first. rewrite translate_first. rewrite subst_app. rewrite subst_first. rewrite IHe. rewrite subst_flush_star. reflexivity.
   + rewrite subst_second. rewrite translate_second. rewrite translate_second. rewrite subst_app. rewrite subst_second. rewrite IHe. rewrite subst_flush_star. reflexivity.
@@ -578,6 +601,583 @@ Proof. intros. induction H; simpl.
   + apply value_lam.
   + apply value_paire. auto. auto. Qed.
 
+Fixpoint remove x l :=
+  match l with
+    | nil => nil
+    | y :: l => if (x =? y) then remove x l else y :: (remove x l)
+end.
+
+Fact remove_id1 : forall y l x, In y l -> y <> x -> In y (remove x l).
+Proof. intros. induction l.
+  + inversion H.
+  + simpl. destruct (x =? a) eqn:ORIG.
+    ++ apply beq_nat_true in ORIG. subst. apply IHl. destruct H. contradiction H0. auto. auto.
+    ++ simpl. destruct H. subst. left. reflexivity. right. apply IHl. auto. Qed.
+
+
+Fact remove_id2 : forall x l, remove x l = nil -> (l = nil \/ (forall y, In y l -> y = x)).
+Proof. intros. induction l.
+  + left. auto.
+  + right. intros. simpl in H. simpl in H0. destruct (x =? a) eqn:ORIG.
+    ++ apply beq_nat_true in ORIG. subst. destruct H0. auto. apply IHl in H. destruct H. subst. inversion H0. apply H. auto.
+    ++ inversion H. Qed.
+
+Fact remove_in_iff : forall x y l, In y (remove x l) <-> ((x=y -> False) /\ (In y l)).
+Proof. intros. unfold iff. split.
+  + intros. generalize dependent x. generalize dependent y. induction l ; intros.
+    ++ inversion H.
+    ++ simpl in H. destruct (x =? a) eqn:ORIG.
+       +++ apply beq_nat_true in ORIG. subst. apply IHl in H. destruct H. split. auto. right. auto.
+       +++ simpl in H. apply beq_nat_false in ORIG. destruct H.
+           ++++ subst. split. auto. left. auto.
+           ++++ apply IHl in H. destruct H. split. auto. right. auto.
+  + intros. apply remove_id1. destruct H. auto. destruct H. auto.
+Qed.
+
+Fixpoint fvs (e : term) : (list nat) :=
+  match e with
+    | array _ => nil
+    | num _ => nil
+    | plus e1 e2 => (fvs e1) ++ (fvs e2)
+    | minus e1 e2 =>  (fvs e1) ++ (fvs e2)
+    | modulo e1 e2 =>  (fvs e1) ++ (fvs e2)
+    | tru => nil
+    | fls => nil
+    | less_than e1 e2 =>  (fvs e1) ++ (fvs e2)
+    | not e => fvs e
+    | and e1 e2 =>  (fvs e1) ++ (fvs e2)
+    | yunit => nil
+    | write e1 e2 e3 => (fvs e1) ++ (fvs e2) ++ (fvs e3)
+    | read e1 e2 =>  (fvs e1) ++ (fvs e2)
+    | reference e => fvs e
+    | cast e => fvs e
+    | case e1 e2 e3 => (fvs e1) ++ (fvs e2) ++ (fvs e3)
+    | var y => y :: nil
+    | app e1 e2 =>  (fvs e1) ++ (fvs e2)
+    | lam e => map (fun x => x - 1) (remove 0 (fvs e))
+    | paire e1 e2 => (fvs e1) ++ (fvs e2)
+    | first e => fvs e
+    | second e => fvs e
+  end.
+
+Fact foo2 : forall n e b, (forall k, In k (fvs e) -> k < n) -> Lambda.shift b n e = e.
+Proof. intros. generalize dependent n. generalize dependent b. induction e ; intros ; simpl in * ; try auto.
+  + rewrite IHe1. rewrite IHe2. auto. intros. apply H. apply in_app_iff. right. auto. intros. apply H. apply in_app_iff. left. auto.
+  + rewrite IHe1. rewrite IHe2. auto. intros. apply H. apply in_app_iff. right. auto. intros. apply H. apply in_app_iff. left. auto.
+  + rewrite IHe1. rewrite IHe2. auto. intros. apply H. apply in_app_iff. right. auto. intros. apply H. apply in_app_iff. left. auto.
+  + rewrite IHe1. rewrite IHe2. auto. intros. apply H. apply in_app_iff. right. auto. intros. apply H. apply in_app_iff. left. auto.
+  + rewrite IHe. auto. auto.
+  + rewrite IHe1. rewrite IHe2. auto. intros. apply H. apply in_app_iff. right. auto. intros. apply H. apply in_app_iff. left. auto.
+  + rewrite IHe1. rewrite IHe2. auto. intros. apply H. apply in_app_iff. right. auto. intros. apply H. apply in_app_iff. left. auto.
+  + rewrite IHe1. rewrite IHe2. rewrite IHe3. auto. intros. apply H. rewrite in_app_iff. rewrite in_app_iff. right. right. auto. intros. apply H. rewrite in_app_iff. rewrite in_app_iff. right. left. auto. intros. apply H. rewrite in_app_iff. left. auto.
+  + rewrite IHe. auto. auto.
+  + rewrite IHe. auto. auto.
+  + rewrite IHe1. rewrite IHe2. rewrite IHe3. auto. intros. apply H. rewrite in_app_iff. rewrite in_app_iff. right. right. auto. intros. apply H. rewrite in_app_iff. rewrite in_app_iff. right. left. auto. intros. apply H. rewrite in_app_iff. left. auto.
+  + destruct (n <? n0) eqn:ORIG.
+    ++ auto.
+    ++ assert (n < n0). apply H. left. auto. apply Nat.ltb_ge in ORIG. omega.
+  + rewrite IHe1. rewrite IHe2. auto. intros. apply H. apply in_app_iff. right. auto. intros. apply H. apply in_app_iff. left. auto.
+  + rewrite IHe. auto. intros. destruct k.
+    ++ omega.
+    ++ assert (k < n). apply H. apply in_map_iff. refine (ex_intro _ (S k) _). split. omega. apply remove_in_iff. split. omega. auto. omega.
+  + rewrite IHe1. rewrite IHe2. auto. intros. apply H. apply in_app_iff. right. auto. intros. apply H. apply in_app_iff. left. auto.
+  + rewrite IHe. auto. auto.
+  + rewrite IHe. auto. auto.
+Qed.
+
+Fact foo3 : forall c k e, c > 0 -> Lambda.shift true k (Lambda.shift false (c+k) e) = Lambda.shift false (c+k+1) (Lambda.shift true k e).
+Proof. intros. generalize dependent c. generalize dependent k. induction e ; intros ; simpl in * ; try auto ; try (rewrite IHe1; try (rewrite IHe2); auto ; auto) ; try (rewrite IHe3 ; auto ; auto) ; try (rewrite IHe ; auto ; auto). destruct (n <? c + k) eqn:ORIG; destruct (n <? k) eqn:ORIG1. replace (n <? c + k + 1) with true. auto. symmetry. apply Nat.ltb_lt. apply Nat.ltb_lt in ORIG. omega. replace (n + 1 <? c+k + 1) with true. auto. symmetry. apply Nat.ltb_lt. apply Nat.ltb_lt in ORIG. omega. destruct (n - 1 <? k) eqn:ORIG2. apply Nat.ltb_ge in ORIG. apply Nat.ltb_lt in ORIG1. omega. replace (n <? c+k+1) with true. apply Nat.ltb_ge in ORIG. assert (n >0). omega. destruct n. omega. simpl. replace (n-0+1) with (S n). auto. omega. symmetry. apply Nat.ltb_lt. apply Nat.ltb_lt in ORIG1. apply Nat.ltb_ge in ORIG. apply Nat.ltb_ge in ORIG2. omega. replace (n+1 <? c+k+1) with false. replace (n - 1 <? k) with false. apply Nat.ltb_ge in ORIG. destruct n. omega. simpl. replace (n-0+1) with (n+1-0). auto. omega. symmetry. apply Nat.ltb_ge. apply Nat.ltb_ge in ORIG. apply Nat.ltb_ge in ORIG1. omega. symmetry. apply Nat.ltb_ge. apply Nat.ltb_ge in ORIG. omega. replace (c+k+1) with (c+(k+1)). rewrite IHe. auto. auto. omega. Qed.
+
+
+Fact foo4 : forall e b k m, k <= m -> ((fvs e = nil) \/ (forall p, In p (fvs e) -> ((p < k) \/ (p >= m)))) -> Lambda.shift b k e = Lambda.shift b m e.
+Proof. intros. generalize dependent k. generalize dependent b.  generalize dependent m. induction e ; intros ; simpl in * ; try auto.
+  + rewrite IHe1 with (m:=m). rewrite IHe2 with (m:=m). auto. auto. 
+    ++ destruct H0.
+       +++ apply app_eq_nil in H0. destruct H0. left. auto.
+       +++ right. intros. apply H0. apply in_or_app. right. auto.
+    ++ auto.
+    ++ destruct H0.
+       +++ apply app_eq_nil in H0. destruct H0. left. auto.
+       +++  right. intros. apply H0. apply in_or_app. left. auto.
+  + rewrite IHe1 with (m:=m). rewrite IHe2 with (m:=m). auto. auto. 
+    ++ destruct H0.
+       +++ apply app_eq_nil in H0. destruct H0. left. auto.
+       +++ right. intros. apply H0. apply in_or_app. right. auto.
+    ++ auto.
+    ++ destruct H0.
+       +++ apply app_eq_nil in H0. destruct H0. left. auto.
+       +++  right. intros. apply H0. apply in_or_app. left. auto.
+  + rewrite IHe1 with (m:=m). rewrite IHe2 with (m:=m). auto. auto. 
+    ++ destruct H0.
+       +++ apply app_eq_nil in H0. destruct H0. left. auto.
+       +++ right. intros. apply H0. apply in_or_app. right. auto.
+    ++ auto.
+    ++ destruct H0.
+       +++ apply app_eq_nil in H0. destruct H0. left. auto.
+       +++  right. intros. apply H0. apply in_or_app. left. auto.
+  + rewrite IHe1 with (m:=m). rewrite IHe2 with (m:=m). auto. auto. 
+    ++ destruct H0.
+       +++ apply app_eq_nil in H0. destruct H0. left. auto.
+       +++ right. intros. apply H0. apply in_or_app. right. auto.
+    ++ auto.
+    ++ destruct H0.
+       +++ apply app_eq_nil in H0. destruct H0. left. auto.
+       +++  right. intros. apply H0. apply in_or_app. left. auto.
+  + rewrite IHe with (m:=m). auto. auto. auto.
+  + rewrite IHe1 with (m:=m). rewrite IHe2 with (m:=m). auto. auto. 
+    ++ destruct H0.
+       +++ apply app_eq_nil in H0. destruct H0. left. auto.
+       +++ right. intros. apply H0. apply in_or_app. right. auto.
+    ++ auto.
+    ++ destruct H0.
+       +++ apply app_eq_nil in H0. destruct H0. left. auto.
+       +++  right. intros. apply H0. apply in_or_app. left. auto.
+  + rewrite IHe1 with (m:=m). rewrite IHe2 with (m:=m). auto. auto. 
+    ++ destruct H0.
+       +++ apply app_eq_nil in H0. destruct H0. left. auto.
+       +++ right. intros. apply H0. apply in_or_app. right. auto.
+    ++ auto.
+    ++ destruct H0.
+       +++ apply app_eq_nil in H0. destruct H0. left. auto.
+       +++  right. intros. apply H0. apply in_or_app. left. auto.
+  + rewrite IHe1 with (m:=m). rewrite IHe2 with (m:=m). rewrite IHe3 with (m:=m). auto. auto. 
+    ++ destruct H0.
+       +++ apply app_eq_nil in H0. destruct H0. apply app_eq_nil in H1. destruct H1. left. auto.
+       +++ right. intros. apply H0. apply in_or_app. right.  apply in_or_app. right. auto.
+    ++ auto.
+    ++ destruct H0.
+       +++ apply app_eq_nil in H0. destruct H0. apply app_eq_nil in H1. destruct H1. left. auto.
+       +++  right. intros. apply H0. apply in_or_app. right. apply in_or_app. left. auto.
+    ++ auto.
+    ++ destruct H0.
+       +++ apply app_eq_nil in H0. destruct H0. left. auto.
+       +++ right. intros. apply H0. apply in_or_app. left. auto.
+  + rewrite IHe with (m:=m). auto. auto. auto.
+  + rewrite IHe with (m:=m). auto. auto. auto.
+  + rewrite IHe1 with (m:=m). rewrite IHe2 with (m:=m). rewrite IHe3 with (m:=m). auto. auto. 
+    ++ destruct H0.
+       +++ apply app_eq_nil in H0. destruct H0. apply app_eq_nil in H1. destruct H1. left. auto.
+       +++ right. intros. apply H0. apply in_or_app. right.  apply in_or_app. right. auto.
+    ++ auto.
+    ++ destruct H0.
+       +++ apply app_eq_nil in H0. destruct H0. apply app_eq_nil in H1. destruct H1. left. auto.
+       +++  right. intros. apply H0. apply in_or_app. right. apply in_or_app. left. auto.
+    ++ auto.
+    ++ destruct H0.
+       +++ apply app_eq_nil in H0. destruct H0. left. auto.
+       +++ right. intros. apply H0. apply in_or_app. left. auto.
+  +  destruct H0.
+    ++ inversion H0.
+    ++ assert (n < k \/ n >= m). apply H0. left. auto. destruct H1.
+       +++ replace (n <? k) with true. replace (n <? m) with true. auto. symmetry. apply Nat.ltb_lt. omega. symmetry. apply Nat.ltb_lt. auto.
+       +++ replace (n <? k) with false. replace (n <? m) with false. auto. symmetry. apply Nat.ltb_ge. omega. symmetry. apply Nat.ltb_ge. omega.
+  + rewrite IHe1 with (m:=m). rewrite IHe2 with (m:=m). auto. auto. 
+    ++ destruct H0.
+       +++ apply app_eq_nil in H0. destruct H0. left. auto.
+       +++ right. intros. apply H0. apply in_or_app. right. auto.
+    ++ auto.
+    ++ destruct H0.
+       +++ apply app_eq_nil in H0. destruct H0. left. auto.
+       +++  right. intros. apply H0. apply in_or_app. left. auto.
+  + rewrite IHe with (m:=m+1). auto. omega. destruct H0. apply map_eq_nil in H0. apply remove_id2 in H0. destruct H0. left. auto. right. intros. assert (p=0). apply H0. auto. subst. left. omega. right. intros. destruct p. left. omega. assert (In p (map (fun x : nat => x - 1) (remove 0 (fvs e)))). apply in_map_iff. refine (ex_intro _ (S p) _). split. omega. apply remove_in_iff. split. omega. auto. apply H0 in H2. destruct H2. left. omega. right. omega.
+  + rewrite IHe1 with (m:=m). rewrite IHe2 with (m:=m). auto. auto. 
+    ++ destruct H0.
+       +++ apply app_eq_nil in H0. destruct H0. left. auto.
+       +++ right. intros. apply H0. apply in_or_app. right. auto.
+    ++ auto.
+    ++ destruct H0.
+       +++ apply app_eq_nil in H0. destruct H0. left. auto.
+       +++  right. intros. apply H0. apply in_or_app. left. auto.
+  + rewrite IHe with (m:=m). auto. auto. auto.
+  + rewrite IHe with (m:=m). auto. auto. auto.
+Qed.
+
+Fact foo5 : forall k e, (In k (fvs e) -> False) -> Lambda.shift true k (Lambda.shift false k e) = Lambda.shift false (k+1) (Lambda.shift true k e).
+Proof. intros. generalize dependent k. induction e ; intros ; simpl in * ; try auto.
+  + rewrite IHe1. rewrite IHe2. auto. intros. contradiction H. apply in_app_iff. right. auto. intros. contradiction H. apply in_app_iff. left. auto.
+  + rewrite IHe1. rewrite IHe2. auto. intros. contradiction H. apply in_app_iff. right. auto. intros. contradiction H. apply in_app_iff. left. auto.
+  + rewrite IHe1. rewrite IHe2. auto. intros. contradiction H. apply in_app_iff. right. auto. intros. contradiction H. apply in_app_iff. left. auto.
+  + rewrite IHe1. rewrite IHe2. auto. intros. contradiction H. apply in_app_iff. right. auto. intros. contradiction H. apply in_app_iff. left. auto.
+  + rewrite IHe. auto. auto.
+  + rewrite IHe1. rewrite IHe2. auto. intros. contradiction H. apply in_app_iff. right. auto. intros. contradiction H. apply in_app_iff. left. auto.
+  + rewrite IHe1. rewrite IHe2. auto. intros. contradiction H. apply in_app_iff. right. auto. intros. contradiction H. apply in_app_iff. left. auto.
+  + rewrite IHe1. rewrite IHe2. rewrite IHe3. auto. intros. apply H. apply in_app_iff. right. apply in_app_iff. right. auto. intros. apply H. apply in_app_iff. right. apply in_app_iff. left. auto. intros. apply H. apply in_app_iff. left. auto.
+  + rewrite IHe. auto. auto.
+  + rewrite IHe. auto. auto.
+  + rewrite IHe1. rewrite IHe2. rewrite IHe3. auto. intros. apply H. apply in_app_iff. right. apply in_app_iff. right. auto. intros. apply H. apply in_app_iff. right. apply in_app_iff. left. auto. intros. apply H. apply in_app_iff. left. auto.
+  + destruct (n <? k) eqn:ORIG.
+    ++ rewrite ORIG. replace (n <? k + 1) with true. auto. symmetry. apply Nat.ltb_lt. apply Nat.ltb_lt in ORIG. omega.
+    ++ replace (n+1 <? k+1) with false. destruct (n-1 <? k) eqn:ORIG2.
+       +++ apply Nat.ltb_lt in ORIG2. apply Nat.ltb_ge in ORIG. assert (n=k). omega. subst. contradiction H. left. auto.
+       +++ destruct n.
+           ++++ simpl in *. apply Nat.ltb_ge in ORIG. assert (k=0). omega. subst. contradiction H. left. auto.
+           ++++ replace (S n-1+1) with (S n + 1 -1). auto. omega.
+       +++ symmetry. apply Nat.ltb_ge. apply Nat.ltb_ge in ORIG. omega.
+  + rewrite IHe1. rewrite IHe2. auto. intros. contradiction H. apply in_app_iff. right. auto. intros. contradiction H. apply in_app_iff. left. auto.
+  + rewrite IHe. auto. intros. rewrite in_map_iff in H. apply H. refine (ex_intro _ (S k) _). split. omega. apply remove_in_iff. split. omega. replace (S k) with (k+1). auto. omega.
+  + rewrite IHe1. rewrite IHe2. auto. intros. contradiction H. apply in_app_iff. right. auto. intros. contradiction H. apply in_app_iff. left. auto.
+  + rewrite IHe. auto. auto.
+  + rewrite IHe. auto. auto.
+Qed.
+
+
+Fact shift_down_seq : forall c e1 e2 , (c = 0 -> (In 0 (fvs e2) -> False)) -> Lambda.shift false c (e1;;e2) = ((Lambda.shift false c e1);;(Lambda.shift false c e2)).
+Proof. intros. unfold seq. rewrite shift_app. rewrite shift_lam. destruct c ; simpl.
+  + assert (In 0 (fvs e2) -> False). apply H. auto. rewrite foo5. auto. auto.
+  + replace (S c) with (c+1+0). rewrite foo3. replace (S (c+1)) with (c+1+0+1). auto. omega. omega. omega. 
+Qed.
+
+Fact fvs_array : forall n, fvs (array n) = nil.
+Proof. intros. simpl. auto. Qed.
+
+Fact fvs_num : forall n, fvs (num n) = nil.
+Proof. intros. simpl. auto. Qed.
+
+Fact fvs_tru : fvs tru = nil.
+Proof. intros. simpl. auto. Qed.
+
+Fact fvs_fls : fvs fls = nil.
+Proof. intros. simpl. auto. Qed.
+
+Fact fvs_plus : forall e1 e2, fvs (plus e1 e2) = (fvs e1) ++ (fvs e2).
+Proof. intros. simpl. auto. Qed.
+
+Fact fvs_minus : forall e1 e2, fvs (minus e1 e2) = (fvs e1) ++ (fvs e2).
+Proof. intros. simpl. auto. Qed.
+
+
+Fact fvs_app : forall e1 e2, fvs (app e1 e2) = (fvs e1) ++ (fvs e2).
+Proof. intros. simpl. auto. Qed.
+Fact fvs_modulo : forall e1 e2, fvs (modulo e1 e2) = (fvs e1) ++ (fvs e2).
+Proof. intros. simpl. auto. Qed.
+Fact fvs_and : forall e1 e2, fvs (and e1 e2) = (fvs e1) ++ (fvs e2).
+Proof. intros. simpl. auto. Qed.
+Fact fvs_less_than : forall e1 e2, fvs (less_than e1 e2) = (fvs e1) ++ (fvs e2).
+Proof. intros. simpl. auto. Qed.
+Fact fvs_paire : forall e1 e2, fvs (paire e1 e2) = (fvs e1) ++ (fvs e2).
+Proof. intros. simpl. auto. Qed.
+Fact fvs_read : forall e1 e2, fvs (read e1 e2) = (fvs e1) ++ (fvs e2).
+Proof. intros. simpl. auto. Qed.
+Fact fvs_case : forall e1 e2 e3, fvs (case e1 e2 e3) = (fvs e1) ++ (fvs e2) ++ (fvs e3).
+Proof. intros. simpl. auto. Qed.
+Fact fvs_write : forall e1 e2 e3, fvs (write e1 e2 e3) = (fvs e1) ++ (fvs e2) ++ (fvs e3).
+Proof. intros. simpl. auto. Qed.
+Fact fvs_not : forall e, fvs (not e) = fvs e.
+Proof. intros. simpl. auto. Qed.
+Fact fvs_reference : forall e, fvs (reference e) = fvs e.
+Proof. intros. simpl. auto. Qed.
+Fact fvs_first : forall e, fvs (first e) = fvs e.
+Proof. intros. simpl. auto. Qed.
+Fact fvs_second : forall e, fvs (second e) = fvs e.
+Proof. intros. simpl. auto. Qed.
+Fact fvs_cast : forall e, fvs (cast e) = fvs e.
+Proof. intros. simpl. auto. Qed.
+Fact fvs_lam : forall e, fvs (lam e) = map (fun x => x - 1) (remove 0 (fvs e)).
+Proof. intros. simpl. auto.
+Qed.
+
+Fact fvs_shift_up : forall c x e, c <= x -> (In (S x) (fvs (Lambda.shift true c e)) <-> In x (fvs e)).
+Proof. intros. generalize dependent c. generalize dependent x. induction e ; intros ; simpl.
+  + intuition.
+  + intuition.
+  + unfold iff. split.
+    ++ intros. apply in_app_iff. apply in_app_iff in H0. destruct H0.
+       +++ left. apply IHe1 in H. apply H. auto.
+       +++ right. apply IHe2 in H. apply H. auto.
+    ++ intros. apply in_app_iff. apply in_app_iff in H0. destruct H0.
+       +++ left. apply IHe1 in H. apply H. auto.
+       +++ right. apply IHe2 in H. apply H. auto.
+  + unfold iff. split.
+    ++ intros. apply in_app_iff. apply in_app_iff in H0. destruct H0.
+       +++ left. apply IHe1 in H. apply H. auto.
+       +++ right. apply IHe2 in H. apply H. auto.
+    ++ intros. apply in_app_iff. apply in_app_iff in H0. destruct H0.
+       +++ left. apply IHe1 in H. apply H. auto.
+       +++ right. apply IHe2 in H. apply H. auto.  + unfold iff. split.
+    ++ intros. apply in_app_iff. apply in_app_iff in H0. destruct H0.
+       +++ left. apply IHe1 in H. apply H. auto.
+       +++ right. apply IHe2 in H. apply H. auto.
+    ++ intros. apply in_app_iff. apply in_app_iff in H0. destruct H0.
+       +++ left. apply IHe1 in H. apply H. auto.
+       +++ right. apply IHe2 in H. apply H. auto.
+  + intuition.
+  + intuition.
+  + unfold iff. split.
+    ++ intros. apply in_app_iff. apply in_app_iff in H0. destruct H0.
+       +++ left. apply IHe1 in H. apply H. auto.
+       +++ right. apply IHe2 in H. apply H. auto.
+    ++ intros. apply in_app_iff. apply in_app_iff in H0. destruct H0.
+       +++ left. apply IHe1 in H. apply H. auto.
+       +++ right. apply IHe2 in H. apply H. auto.
+  + apply IHe in H. auto.
+  + unfold iff. split.
+    ++ intros. apply in_app_iff. apply in_app_iff in H0. destruct H0.
+       +++ left. apply IHe1 in H. apply H. auto.
+       +++ right. apply IHe2 in H. apply H. auto.
+    ++ intros. apply in_app_iff. apply in_app_iff in H0. destruct H0.
+       +++ left. apply IHe1 in H. apply H. auto.
+       +++ right. apply IHe2 in H. apply H. auto.
+  + intuition.
+  + unfold iff. split.
+    ++ intros. apply in_app_iff. apply in_app_iff in H0. destruct H0.
+       +++ left. apply IHe1 in H. apply H. auto.
+       +++ right. apply IHe2 in H. apply H. auto.
+    ++ intros. apply in_app_iff. apply in_app_iff in H0. destruct H0.
+       +++ left. apply IHe1 in H. apply H. auto.
+       +++ right. apply IHe2 in H. apply H. auto.
+  + unfold iff. split.
+    ++ intros. apply in_app_iff. apply in_app_iff in H0. destruct H0.
+       +++ left. apply IHe1 in H. apply H. auto.
+       +++ apply in_app_iff in H0. destruct H0. right. apply IHe2 in H. apply in_app_iff. left. apply H. auto. apply IHe3 in H. right. apply in_app_iff. right. apply H. auto.
+    ++ intros. apply in_app_iff. apply in_app_iff in H0. destruct H0.
+       +++ left. apply IHe1 in H. apply H. auto.
+       +++ apply in_app_iff in H0. destruct H0. right. apply IHe2 in H. apply in_app_iff. left. apply H. auto. apply IHe3 in H. right. apply in_app_iff. right. apply H. auto.
+  + apply IHe in H. auto.
+  + apply IHe in H. auto.
+  +  unfold iff. split.
+    ++ intros. apply in_app_iff. apply in_app_iff in H0. destruct H0.
+       +++ left. apply IHe1 in H. apply H. auto.
+       +++ right. apply in_app_iff in H0. destruct H0.
+           ++++ apply IHe2 in H. apply in_app_iff. left. apply H. auto.
+           ++++ apply IHe3 in H. apply in_app_iff. right. apply H. auto.
+    ++ intros. apply in_app_iff. apply in_app_iff in H0. destruct H0.
+       +++ left. apply IHe1 in H. apply H. auto.
+       +++ right. apply in_app_iff in H0. destruct H0.
+           ++++ apply IHe2 in H. apply in_app_iff. left. apply H. auto.
+           ++++ apply IHe3 in H. apply in_app_iff. right. apply H. auto.
+  + unfold iff. split. 
+    ++ intros. destruct (n <? c) eqn:ORIG.
+       +++ apply Nat.ltb_lt in ORIG. destruct H0.
+           ++++ subst. omega.
+           ++++ contradiction H0.
+       +++ destruct H0.
+           ++++ left. omega.
+           ++++ contradiction H0.
+    ++ intros. destruct (n <? c) eqn:ORIG.
+       +++ apply Nat.ltb_lt in ORIG. destruct H0.
+           ++++ subst. omega.
+           ++++ contradiction H0.
+       +++ destruct H0.
+           ++++ left. omega.
+           ++++ contradiction H0.
+  + unfold iff. split.
+    ++ intros. apply in_app_iff. apply in_app_iff in H0. destruct H0.
+       +++ left. apply IHe1 in H. apply H. auto.
+       +++ right. apply IHe2 in H. apply H. auto.
+    ++ intros. apply in_app_iff. apply in_app_iff in H0. destruct H0.
+       +++ left. apply IHe1 in H. apply H. auto.
+       +++ right. apply IHe2 in H. apply H. auto.
+  + unfold iff. split.
+    ++ intros. apply in_map_iff. apply in_map_iff in H0. destruct H0. destruct H0. apply remove_in_iff in H1. destruct H1. replace x0 with (S (S x)) in *. apply IHe in H2. refine (ex_intro _ (S x) _). split. omega. apply remove_in_iff. split. omega. auto. omega. omega.
+    ++ intros. intros. apply in_map_iff. apply in_map_iff in H0. destruct H0. destruct H0. apply remove_in_iff in H1. destruct H1. replace x0 with ((S x)) in *. assert (S c <= S x). omega. apply IHe in H3. refine (ex_intro _ (S (S x)) _ ). split. omega. apply remove_in_iff. split. omega. replace (S c) with (c+1) in *. apply H3. auto. omega. omega.
+  + unfold iff. split.
+    ++ intros. apply in_app_iff. apply in_app_iff in H0. destruct H0.
+       +++ left. apply IHe1 in H. apply H. auto.
+       +++ right. apply IHe2 in H. apply H. auto.
+    ++ intros. apply in_app_iff. apply in_app_iff in H0. destruct H0.
+       +++ left. apply IHe1 in H. apply H. auto.
+       +++ right. apply IHe2 in H. apply H. auto.
+  + apply IHe in H. auto.
+  + apply IHe in H. auto.
+Qed.
+
+Fact fvs_translate : forall e thread base buf_size, (forall x, In x (fvs e) <-> In x (fvs (translate e thread base buf_size))).
+Proof. intros. generalize dependent x. induction e ; intros.
+  + simpl. intuition.
+  + simpl. intuition.
+  + rewrite translate_plus. rewrite fvs_plus. rewrite fvs_app. unfold iff. split.
+    ++ intros. destruct thread.
+       +++ simpl. apply in_app_iff in H. destruct H. apply in_app_iff. left. apply IHe1. auto. apply in_app_iff. right. apply IHe2. auto.
+       +++ simpl. apply in_app_iff in H. destruct H. apply in_app_iff. left. apply IHe1. auto. apply in_app_iff. right. apply IHe2. auto.
+    ++ intros. destruct thread.
+       +++ simpl in *. apply in_app_iff. apply in_app_iff in H. destruct H.
+           ++++ left. apply IHe1. auto.
+           ++++ right. apply IHe2. auto.
+       +++ simpl in *. apply in_app_iff. apply in_app_iff in H. destruct H.
+           ++++ left. apply IHe1. auto.
+           ++++ right. apply IHe2. auto.
+  + rewrite translate_minus. rewrite fvs_minus. rewrite fvs_app. unfold iff. split.
+    ++ intros. destruct thread.
+       +++ simpl. apply in_app_iff in H. destruct H. apply in_app_iff. left. apply IHe1. auto. apply in_app_iff. right. apply IHe2. auto.
+       +++ simpl. apply in_app_iff in H. destruct H. apply in_app_iff. left. apply IHe1. auto. apply in_app_iff. right. apply IHe2. auto.
+    ++ intros. destruct thread.
+       +++ simpl in *. apply in_app_iff. apply in_app_iff in H. destruct H.
+           ++++ left. apply IHe1. auto.
+           ++++ right. apply IHe2. auto.
+       +++ simpl in *. apply in_app_iff. apply in_app_iff in H. destruct H.
+           ++++ left. apply IHe1. auto.
+           ++++ right. apply IHe2. auto.
+  + rewrite translate_modulo. rewrite fvs_modulo. rewrite fvs_app. unfold iff. split.
+    ++ intros. destruct thread.
+       +++ simpl. apply in_app_iff in H. destruct H. apply in_app_iff. left. apply IHe1. auto. apply in_app_iff. right. apply IHe2. auto.
+       +++ simpl. apply in_app_iff in H. destruct H. apply in_app_iff. left. apply IHe1. auto. apply in_app_iff. right. apply IHe2. auto.
+    ++ intros. destruct thread.
+       +++ simpl in *. apply in_app_iff. apply in_app_iff in H. destruct H.
+           ++++ left. apply IHe1. auto.
+           ++++ right. apply IHe2. auto.
+       +++ simpl in *. apply in_app_iff. apply in_app_iff in H. destruct H.
+           ++++ left. apply IHe1. auto.
+           ++++ right. apply IHe2. auto.
+  + simpl. intuition.
+  + simpl. intuition.
+  + rewrite translate_less_than. rewrite fvs_less_than. rewrite fvs_app. unfold iff. split.
+    ++ intros. destruct thread.
+       +++ simpl. apply in_app_iff in H. destruct H. apply in_app_iff. left. apply IHe1. auto. apply in_app_iff. right. apply IHe2. auto.
+       +++ simpl. apply in_app_iff in H. destruct H. apply in_app_iff. left. apply IHe1. auto. apply in_app_iff. right. apply IHe2. auto.
+    ++ intros. destruct thread.
+       +++ simpl in *. apply in_app_iff. apply in_app_iff in H. destruct H.
+           ++++ left. apply IHe1. auto.
+           ++++ right. apply IHe2. auto.
+       +++ simpl in *. apply in_app_iff. apply in_app_iff in H. destruct H.
+           ++++ left. apply IHe1. auto.
+           ++++ right. apply IHe2. auto.
+  + rewrite translate_not. rewrite fvs_not. rewrite fvs_app. unfold iff. split.
+    ++ intros. destruct thread.
+       +++ simpl. apply IHe. auto.
+       +++ simpl. apply IHe. auto.
+    ++ intros. destruct thread.
+       +++ simpl in H. apply IHe. auto.
+       +++ simpl in H. apply IHe. auto.
+  + rewrite translate_and. rewrite fvs_and. rewrite fvs_app. unfold iff. split.
+    ++ intros. destruct thread.
+       +++ simpl. apply in_app_iff in H. destruct H. apply in_app_iff. left. apply IHe1. auto. apply in_app_iff. right. apply IHe2. auto.
+       +++ simpl. apply in_app_iff in H. destruct H. apply in_app_iff. left. apply IHe1. auto. apply in_app_iff. right. apply IHe2. auto.
+    ++ intros. destruct thread.
+       +++ simpl in *. apply in_app_iff. apply in_app_iff in H. destruct H.
+           ++++ left. apply IHe1. auto.
+           ++++ right. apply IHe2. auto.
+       +++ simpl in *. apply in_app_iff. apply in_app_iff in H. destruct H.
+           ++++ left. apply IHe1. auto.
+           ++++ right. apply IHe2. auto.
+  + simpl. intuition.
+  + rewrite translate_read. rewrite fvs_read. rewrite fvs_app. unfold new_read. rewrite fvs_app. unfold iff. split.
+    ++ intros. destruct thread.
+       +++ simpl. apply in_app_iff in H. destruct H. apply in_app_iff. left. apply IHe1. auto. apply in_app_iff. right. apply IHe2. auto.
+       +++ simpl. apply in_app_iff in H. destruct H. apply in_app_iff. left. apply IHe1. auto. apply in_app_iff. right. apply IHe2. auto.
+    ++ intros. destruct thread.
+       +++ simpl in *. apply in_app_iff. apply in_app_iff in H. destruct H.
+           ++++ left. apply IHe1. auto.
+           ++++ right. apply IHe2. auto.
+       +++ simpl in *. apply in_app_iff. apply in_app_iff in H. destruct H.
+           ++++ left. apply IHe1. auto.
+           ++++ right. apply IHe2. auto.
+  + rewrite translate_write. rewrite fvs_write. rewrite fvs_app. unfold new_write. rewrite fvs_app. rewrite fvs_paire. rewrite fvs_paire. unfold iff. split.
+    ++ intros. destruct thread.
+       +++ simpl. apply in_app_iff in H. destruct H. apply in_app_iff. left. apply IHe1. auto. apply in_app_iff. right. apply in_app_iff in H. destruct H. apply in_app_iff. left. apply IHe2. auto. apply in_app_iff. right. apply IHe3. auto.
+       +++ simpl. simpl. apply in_app_iff in H. destruct H. apply in_app_iff. left. apply IHe1. auto. apply in_app_iff. right. apply in_app_iff in H. destruct H. apply in_app_iff. left. apply IHe2. auto. apply in_app_iff. right. apply IHe3. auto.
+    ++ intros. destruct thread.
+       +++ simpl in *. apply in_app_iff. apply in_app_iff in H. destruct H.
+           ++++ left. apply IHe1. auto.
+           ++++ apply in_app_iff in H. destruct H. right. apply in_app_iff. left. apply IHe2. auto. right. apply in_app_iff. right. apply IHe3. auto.
+       +++ simpl in *. apply in_app_iff. apply in_app_iff in H. destruct H.
+           ++++ left. apply IHe1. auto.
+           ++++ apply in_app_iff in H. destruct H. right. apply in_app_iff. left. apply IHe2. auto. right. apply in_app_iff. right. apply IHe3. auto.
+  + rewrite translate_reference. rewrite fvs_reference. rewrite fvs_app. unfold iff. split.
+    ++ intros. destruct thread.
+       +++ simpl. apply IHe. auto.
+       +++ simpl. apply IHe. auto.
+    ++ intros. destruct thread.
+       +++ simpl in H. apply IHe. auto.
+       +++ simpl in H. apply IHe. auto.
+  + rewrite translate_cast. rewrite fvs_cast. rewrite fvs_app. unfold iff. split.
+    ++ intros. destruct thread.
+       +++ simpl. apply IHe. auto.
+       +++ simpl. apply IHe. auto.
+    ++ intros. destruct thread.
+       +++ simpl in H. apply IHe. auto.
+       +++ simpl in H. apply IHe. auto.
+  + rewrite translate_case. rewrite fvs_case. unfold iff. split.
+    ++ intros. destruct thread.
+       +++ simpl. apply in_app_iff in H. destruct H. apply in_app_iff. left. apply IHe1. auto. apply in_app_iff. right. apply in_app_iff in H. destruct H. apply in_app_iff. left. apply in_app_iff. left. apply in_map_iff. refine (ex_intro _ (S x) _). split. omega. apply remove_in_iff. split. omega. apply fvs_shift_up. omega. apply IHe2. auto. apply in_app_iff. right. apply in_app_iff. left. apply in_map_iff. refine (ex_intro _ (S x) _). split. omega. apply remove_in_iff. split. omega. apply fvs_shift_up. omega. apply IHe3. auto.
+        +++ simpl. apply in_app_iff in H. destruct H. apply in_app_iff. left. apply IHe1. auto. apply in_app_iff. right. apply in_app_iff in H. destruct H. apply in_app_iff. left. apply in_app_iff. left. apply in_map_iff. refine (ex_intro _ (S x) _). split. omega. apply remove_in_iff. split. omega. apply fvs_shift_up. omega. apply IHe2. auto. apply in_app_iff. right. apply in_app_iff. left. apply in_map_iff. refine (ex_intro _ (S x) _). split. omega. apply remove_in_iff. split. omega. apply fvs_shift_up. omega. apply IHe3. auto.
+     ++ intros. destruct thread.
+        +++ simpl in H. apply in_app_iff in H. destruct H.
+            ++++ apply in_app_iff. left. apply IHe1. auto.
+            ++++ apply in_app_iff in H. destruct H.
+                 +++++ apply in_app_iff in H. destruct H. apply in_map_iff in H. destruct H. destruct H. subst. apply remove_in_iff in H0. destruct H0. assert (exists x, x0 = S x). destruct x0. omega. refine (ex_intro _ x0 _). auto. destruct H1. subst. replace (S x - 1) with x. apply in_app_iff. right. apply in_app_iff. left. apply fvs_shift_up in H0. apply IHe2. auto. omega. omega. inversion H.
+                 +++++ apply in_app_iff in H. destruct H. apply in_map_iff in H. destruct H. destruct H. subst. apply remove_in_iff in H0. destruct H0. assert (exists x, x0 = S x). destruct x0. omega. refine (ex_intro _ x0 _). auto. destruct H1. subst. replace (S x - 1) with x. apply in_app_iff. right. apply in_app_iff. right. apply fvs_shift_up in H0. apply IHe3. auto. omega. omega. inversion H.
++++ simpl in H. apply in_app_iff in H. destruct H.
+            ++++ apply in_app_iff. left. apply IHe1. auto.
+            ++++ apply in_app_iff in H. destruct H.
+                 +++++ apply in_app_iff in H. destruct H. apply in_map_iff in H. destruct H. destruct H. subst. apply remove_in_iff in H0. destruct H0. assert (exists x, x0 = S x). destruct x0. omega. refine (ex_intro _ x0 _). auto. destruct H1. subst. replace (S x - 1) with x. apply in_app_iff. right. apply in_app_iff. left. apply fvs_shift_up in H0. apply IHe2. auto. omega. omega. inversion H.
+                 +++++ apply in_app_iff in H. destruct H. apply in_map_iff in H. destruct H. destruct H. subst. apply remove_in_iff in H0. destruct H0. assert (exists x, x0 = S x). destruct x0. omega. refine (ex_intro _ x0 _). auto. destruct H1. subst. replace (S x - 1) with x. apply in_app_iff. right. apply in_app_iff. right. apply fvs_shift_up in H0. apply IHe3. auto. omega. omega. inversion H.
+  + simpl. intuition.
+  + rewrite translate_app. rewrite fvs_app. rewrite fvs_app. unfold iff. split.
+    ++ intros. destruct thread.
+       +++ simpl. apply in_app_iff in H. destruct H. apply in_app_iff. left. apply IHe1. auto. apply in_app_iff. right. apply IHe2. auto.
+       +++ simpl. apply in_app_iff in H. destruct H. apply in_app_iff. left. apply IHe1. auto. apply in_app_iff. right. apply IHe2. auto.
+    ++ intros. destruct thread.
+       +++ simpl in *. apply in_app_iff. apply in_app_iff in H. destruct H.
+           ++++ left. apply IHe1. auto.
+           ++++ right. apply IHe2. auto.
+       +++ simpl in *. apply in_app_iff. apply in_app_iff in H. destruct H.
+           ++++ left. apply IHe1. auto.
+           ++++ right. apply IHe2. auto.
+  + rewrite translate_lam. rewrite fvs_lam. rewrite fvs_lam. rewrite in_map_iff. rewrite in_map_iff. unfold iff. split.
+    ++ intros. destruct thread.
+       +++ simpl. destruct H. destruct H. subst. apply remove_in_iff in H0. destruct H0. destruct x0. omega. refine (ex_intro _ (S x0) _). split. auto. apply remove_in_iff. split. omega. apply in_app_iff. left. apply in_map_iff. refine (ex_intro _ (S (S x0)) _ ). split. omega. apply remove_in_iff. split. omega. admit.
+       +++ simpl. destruct H. destruct H. subst. apply remove_in_iff in H0. destruct H0. destruct x0. omega. refine (ex_intro _ (S x0) _). split. auto. apply remove_in_iff. split. omega. apply in_app_iff. left. apply in_map_iff. refine (ex_intro _ (S (S x0)) _ ). split. omega. apply remove_in_iff. split. omega. admit.
+    ++ intros. destruct thread.
+       +++ simpl in H. destruct H. destruct H. subst. apply remove_in_iff in H0. destruct H0. destruct x0. omega. refine (ex_intro _ (S x0) _). split. auto. apply remove_in_iff. split. omega. apply in_app_iff in H0. destruct H0.
+           ++++ apply in_map_iff in H0. destruct H0. destruct H0. assert (x=S (S x0)). omega. subst. apply remove_in_iff in H1. destruct H1. admit.
+           ++++ inversion H0.
+       +++ simpl in H. destruct H. destruct H. subst. apply remove_in_iff in H0. destruct H0. destruct x0. omega. refine (ex_intro _ (S x0) _). split. auto. apply remove_in_iff. split. omega. apply in_app_iff in H0. destruct H0.
+           ++++ apply in_map_iff in H0. destruct H0. destruct H0. assert (x=S (S x0)). omega. subst. apply remove_in_iff in H1. destruct H1. admit.
+           ++++ inversion H0.
+  + rewrite translate_paire. rewrite fvs_paire. rewrite fvs_paire. unfold iff. split.
+    ++ intros. destruct thread.
+       +++ simpl. apply in_app_iff in H. destruct H. apply in_app_iff. left. apply IHe1. auto. apply in_app_iff. right. apply IHe2. auto.
+       +++ simpl. apply in_app_iff in H. destruct H. apply in_app_iff. left. apply IHe1. auto. apply in_app_iff. right. apply IHe2. auto.
+    ++ intros. destruct thread.
+       +++ simpl in *. apply in_app_iff. apply in_app_iff in H. destruct H.
+           ++++ left. apply IHe1. auto.
+           ++++ right. apply IHe2. auto.
+       +++ simpl in *. apply in_app_iff. apply in_app_iff in H. destruct H.
+           ++++ left. apply IHe1. auto.
+           ++++ right. apply IHe2. auto.
+  + rewrite translate_first. rewrite fvs_first. rewrite fvs_app. unfold iff. split.
+    ++ intros. destruct thread.
+       +++ simpl. apply IHe. auto.
+       +++ simpl. apply IHe. auto.
+    ++ intros. destruct thread.
+       +++ simpl in H. apply IHe. auto.
+       +++ simpl in H. apply IHe. auto.
+  + rewrite translate_second. rewrite fvs_second. rewrite fvs_app. unfold iff. split.
+    ++ intros. destruct thread.
+       +++ simpl. apply IHe. auto.
+       +++ simpl. apply IHe. auto.
+    ++ intros. destruct thread.
+       +++ simpl in H. apply IHe. auto.
+       +++ simpl in H. apply IHe. auto.
+Admitted.
+
+
+
+
+Fact shift_down_commutes_with_translate : forall c e thread base buf_size, (c = 0 -> (In 0 (fvs e) -> False)) -> translate (Lambda.shift false c e) thread base buf_size = Lambda.shift false c (translate e thread base buf_size).
+Proof. intros. generalize dependent c; induction e ; intros.
+  + simpl. auto.
+  + simpl. auto.
+  + rewrite shift_plus. rewrite translate_plus. rewrite translate_plus. rewrite shift_app. rewrite shift_plus. rewrite shift_lam. rewrite shift_down_seq. rewrite shift_flush_star1. rewrite IHe1. rewrite IHe2. destruct c; simpl ; auto. intros. apply H. auto. simpl. apply in_app_iff. right. auto. intros. apply H. auto. simpl. apply in_app_iff. left. auto. intros. omega.
+  + rewrite shift_minus. rewrite translate_minus. rewrite translate_minus. rewrite shift_app. rewrite shift_minus. rewrite shift_lam. rewrite shift_down_seq. rewrite shift_flush_star1. rewrite IHe1. rewrite IHe2. simpl. destruct c; simpl ; auto. intros. apply H. auto. simpl. apply in_app_iff. right. auto. intros. apply H. auto. simpl. apply in_app_iff. left. auto. intros. omega.
+  + rewrite shift_modulo. rewrite translate_modulo. rewrite translate_modulo. rewrite shift_app. rewrite shift_modulo. rewrite shift_lam. rewrite shift_down_seq. rewrite shift_flush_star1. rewrite IHe1. rewrite IHe2. destruct c; simpl ; auto. intros. apply H. auto. simpl. apply in_app_iff. right. auto. intros. apply H. auto. simpl. apply in_app_iff. left. auto. intros. omega.
+  + simpl. auto.
+  + simpl. auto.
+  + rewrite shift_less_than. rewrite translate_less_than. rewrite translate_less_than. rewrite shift_app. rewrite shift_less_than. rewrite shift_lam. rewrite shift_down_seq. rewrite shift_flush_star1. rewrite IHe1. rewrite IHe2. destruct c; simpl ; auto. intros. apply H. auto. simpl. apply in_app_iff. right. auto. intros. apply H. auto. simpl. apply in_app_iff. left. auto. intros. omega.
+  + rewrite shift_not. rewrite translate_not. rewrite translate_not. rewrite shift_app. rewrite shift_not. rewrite shift_lam. rewrite shift_down_seq. rewrite shift_flush_star1. rewrite IHe. destruct c; simpl ; auto. simpl in H. auto. intros. omega.
+  + rewrite shift_and. rewrite translate_and. rewrite translate_and. rewrite shift_app. rewrite shift_and. rewrite shift_lam. rewrite shift_down_seq. rewrite shift_flush_star1. rewrite IHe1. rewrite IHe2. simpl. destruct c; simpl ; auto. intros. apply H. auto. simpl. apply in_app_iff. right. auto. intros. apply H. auto. simpl. apply in_app_iff. left. auto. intros. omega.
+  + simpl. auto.
+  + rewrite shift_read. rewrite translate_read. rewrite translate_read. rewrite shift_app. rewrite IHe1. rewrite IHe2. rewrite shift_new_read_star1. rewrite shift_lam. rewrite shift_down_seq. rewrite shift_flush_star1. destruct c; simpl ; auto. intros. omega. intros. apply H. auto. simpl. apply in_app_iff. right. auto. intros. apply H. auto. simpl. apply in_app_iff. left. auto.
+  + rewrite shift_write. rewrite translate_write. rewrite translate_write. rewrite shift_app. rewrite IHe1. rewrite IHe2. rewrite IHe3. rewrite shift_new_write_star1. rewrite shift_lam. rewrite shift_down_seq. rewrite shift_flush_star1. simpl (Lambda.shift true (0 + 1) (var 0)). destruct c; simpl ; auto. intros. omega. intros. apply H. auto. simpl. apply in_app_iff. right. apply in_app_iff. right. auto. intros. auto. apply H. auto. simpl. apply in_app_iff. right. apply in_app_iff. left. auto. intros. apply H. auto. simpl. apply in_app_iff. left. auto.
+  + rewrite shift_reference. rewrite translate_reference. rewrite translate_reference. rewrite shift_app. rewrite shift_reference. rewrite shift_lam. rewrite shift_down_seq. rewrite shift_flush_star1. rewrite IHe. destruct c; simpl ; auto. simpl in H. auto. intros. omega.
+  + rewrite shift_cast. rewrite translate_cast. rewrite translate_cast. rewrite shift_app. rewrite shift_cast. rewrite shift_lam. rewrite shift_down_seq. rewrite shift_flush_star1. rewrite IHe. destruct c; simpl ; auto. simpl in H. auto. intros. omega.
+  + rewrite shift_case. rewrite translate_case. rewrite translate_case. rewrite shift_case. rewrite IHe1. rewrite IHe2. rewrite IHe3. rewrite shift_down_seq. rewrite shift_flush_star1. rewrite shift_down_seq. rewrite shift_flush_star1. destruct c; simpl ; auto. admit. admit. intros. apply H. auto. simpl. apply in_app_iff. right. apply in_app_iff. right. auto. intros. auto. apply H. auto. simpl. apply in_app_iff. right. apply in_app_iff. left. auto. intros. apply H. auto. simpl. apply in_app_iff. left. auto.
+  + simpl. auto.
+  + rewrite shift_app. rewrite translate_app. rewrite translate_app. rewrite shift_app. rewrite IHe1. rewrite IHe2. destruct c; simpl ; auto. intros. apply H. auto. simpl. apply in_app_iff. right. auto. intros. apply H. auto. simpl. apply in_app_iff. left. auto.
+  + rewrite shift_lam. rewrite translate_lam. rewrite translate_lam. rewrite shift_lam. rewrite shift_down_seq. rewrite shift_flush_star1. rewrite IHe. auto. intros. omega. intros. omega.
+  + rewrite shift_paire. rewrite translate_paire. rewrite translate_paire. rewrite shift_paire. rewrite IHe1. rewrite IHe2. destruct c; simpl ; auto. intros. apply H. auto. simpl. apply in_app_iff. right. auto. intros. apply H. auto. simpl. apply in_app_iff. left. auto.
+  + rewrite shift_first. rewrite translate_first. rewrite translate_first. rewrite shift_app. rewrite shift_first. rewrite shift_lam. rewrite shift_down_seq. rewrite shift_flush_star1. rewrite IHe. destruct c; simpl ; auto. simpl in H. auto. intros. omega.
+  + rewrite shift_second. rewrite translate_second. rewrite translate_second. rewrite shift_app. rewrite shift_second. rewrite shift_lam. rewrite shift_down_seq. rewrite shift_flush_star1. rewrite IHe. destruct c; simpl ; auto.  simpl in H. auto. intros. omega. Admitted.
 
 Fact translation_of_context_steps : forall e e' b B buf_size f m' m'0 l l' thread E u v u' v',
 (forall t, u t = if thread_equals t thread then translate e b B buf_size else f t) ->
